low ~ mid

src/specs/permutationQuotientContribution.ec
@@ -1,111 +1,390 @@
 pragma Goals:printall.
 
 require import AllCore Int IntDiv.
-require import Constants Field Verifier UInt256 YulPrimops PurePrimops VerifierConsts.
+require import Constants Field Verifier Memory UInt256 YulPrimops PurePrimops VerifierConsts.
 
-module PermutationQuotientContribution = {
+theory PermutationQuotientContribution.
 
-  proc low(): uint256 = {
-    var usr_res, a4, zperm_zo, usr_gamma, usr_beta, usr_factorMultiplier, sigma0_z, a_z, sigma1_z, b_z, sigma2_z, c_z, sigma3_z, _22, l0AtZ, a5, _26;
-    a4 <@ Primops.mload(STATE_POWER_OF_ALPHA_4_SLOT);
-    zperm_zo <@ Primops.mload(PROOF_COPY_PERMUTATION_GRAND_PRODUCT_OPENING_AT_Z_OMEGA_SLOT);
-    usr_res <- (PurePrimops.mulmod a4 zperm_zo (W256.of_int R));
-    
+import MemoryMap.
+
+op memory : mem.
+pred in_mem (c : uint256) (v : int) = W256.to_uint (PurePrimops.mload memory c) = v.
+
+op Alpha4 : int.
+op Alpha5 : int. 
+op Gamma : int. 
+op Beta  : int.
+op sigma0_z : int. 
+op sigma1_z : int. 
+op sigma2_z : int. 
+op sigma3_z : int. 
+op a_z : int. 
+op b_z : int. 
+op c_z : int. 
+op zperm_zO : int. 
+op l0_z : int. 
+
+axiom alpha4_mem : in_mem STATE_POWER_OF_ALPHA_4_SLOT Alpha4.
+axiom alpha5_mem : in_mem STATE_POWER_OF_ALPHA_5_SLOT Alpha5.
+axiom gamma_mem : in_mem STATE_GAMMA_SLOT Gamma.
+axiom beta_mem  : in_mem STATE_BETA_SLOT Beta.
+axiom sigma0_z_mem : in_mem PROOF_COPY_PERMUTATION_POLYS_0_OPENING_AT_Z_SLOT sigma0_z.
+axiom sigma1_z_mem : in_mem PROOF_COPY_PERMUTATION_POLYS_1_OPENING_AT_Z_SLOT sigma1_z.
+axiom sigma2_z_mem : in_mem PROOF_COPY_PERMUTATION_POLYS_2_OPENING_AT_Z_SLOT sigma2_z.
+axiom sigma3_z_mem : in_mem PROOF_STATE_POLYS_3_OPENING_AT_Z_SLOT sigma3_z.
+axiom a_z_mem : in_mem PROOF_STATE_POLYS_0_OPENING_AT_Z_SLOT a_z.
+axiom b_z_mem : in_mem PROOF_STATE_POLYS_1_OPENING_AT_Z_SLOT b_z.
+axiom c_z_mem : in_mem PROOF_STATE_POLYS_2_OPENING_AT_Z_SLOT c_z.
+axiom zperm_zO_mem : in_mem PROOF_COPY_PERMUTATION_GRAND_PRODUCT_OPENING_AT_Z_OMEGA_SLOT zperm_zO.
+axiom l0_z_mem : in_mem STATE_L_0_AT_Z_SLOT l0_z.
+
+module M = {
+
+  proc low0(): uint256 = {
+    var usr_res, tmp270, tmp271, usr_gamma, usr_beta, usr_factorMultiplier, tmp274, tmp275, tmp276, tmp277, tmp278, tmp279, tmp280, _22, usr_l0AtZ, tmp282, _26;
+    tmp270 <@ Primops.mload(STATE_POWER_OF_ALPHA_4_SLOT);
+    tmp271 <@ Primops.mload(PROOF_COPY_PERMUTATION_GRAND_PRODUCT_OPENING_AT_Z_OMEGA_SLOT);
+    usr_res <- (PurePrimops.mulmod tmp271 tmp270 (W256.of_int R));
     usr_gamma <@ Primops.mload(STATE_GAMMA_SLOT);
     usr_beta <@ Primops.mload(STATE_BETA_SLOT);
-    
-    sigma0_z <@ Primops.mload(PROOF_COPY_PERMUTATION_POLYS_0_OPENING_AT_Z_SLOT);
-    usr_factorMultiplier <- (PurePrimops.mulmod sigma0_z usr_beta (W256.of_int R));
+    tmp274 <@ Primops.mload(PROOF_COPY_PERMUTATION_POLYS_0_OPENING_AT_Z_SLOT);
+    usr_factorMultiplier <- (PurePrimops.mulmod tmp274 usr_beta (W256.of_int R));
     usr_factorMultiplier <- (PurePrimops.addmod usr_factorMultiplier usr_gamma (W256.of_int R));
-    a_z <@ Primops.mload(PROOF_STATE_POLYS_0_OPENING_AT_Z_SLOT);
-    usr_factorMultiplier <- (PurePrimops.addmod usr_factorMultiplier a_z (W256.of_int R));
+    tmp275 <@ Primops.mload(PROOF_STATE_POLYS_0_OPENING_AT_Z_SLOT);
+    usr_factorMultiplier <- (PurePrimops.addmod usr_factorMultiplier tmp275 (W256.of_int R));
     usr_res <- (PurePrimops.mulmod usr_res usr_factorMultiplier (W256.of_int R));
-    
-    sigma1_z <@ Primops.mload(PROOF_COPY_PERMUTATION_POLYS_1_OPENING_AT_Z_SLOT);
-    usr_factorMultiplier <- (PurePrimops.mulmod sigma1_z usr_beta (W256.of_int R));
+    tmp276 <@ Primops.mload(PROOF_COPY_PERMUTATION_POLYS_1_OPENING_AT_Z_SLOT);
+    usr_factorMultiplier <- (PurePrimops.mulmod tmp276 usr_beta (W256.of_int R));
     usr_factorMultiplier <- (PurePrimops.addmod usr_factorMultiplier usr_gamma (W256.of_int R));
-    b_z <@ Primops.mload(PROOF_STATE_POLYS_1_OPENING_AT_Z_SLOT);
-    usr_factorMultiplier <- (PurePrimops.addmod usr_factorMultiplier b_z (W256.of_int R));
+    tmp277 <@ Primops.mload(PROOF_STATE_POLYS_1_OPENING_AT_Z_SLOT);
+    usr_factorMultiplier <- (PurePrimops.addmod usr_factorMultiplier tmp277 (W256.of_int R));
     usr_res <- (PurePrimops.mulmod usr_res usr_factorMultiplier (W256.of_int R));
-    
-    sigma2_z <@ Primops.mload(PROOF_COPY_PERMUTATION_POLYS_2_OPENING_AT_Z_SLOT);
-    usr_factorMultiplier <- (PurePrimops.mulmod sigma2_z usr_beta (W256.of_int R));
+    tmp278 <@ Primops.mload(PROOF_COPY_PERMUTATION_POLYS_2_OPENING_AT_Z_SLOT);
+    usr_factorMultiplier <- (PurePrimops.mulmod tmp278 usr_beta (W256.of_int R));
     usr_factorMultiplier <- (PurePrimops.addmod usr_factorMultiplier usr_gamma (W256.of_int R));
-    c_z <@ Primops.mload(PROOF_STATE_POLYS_2_OPENING_AT_Z_SLOT);
-    usr_factorMultiplier <- (PurePrimops.addmod usr_factorMultiplier c_z (W256.of_int R));
+    tmp279 <@ Primops.mload(PROOF_STATE_POLYS_2_OPENING_AT_Z_SLOT);
+    usr_factorMultiplier <- (PurePrimops.addmod usr_factorMultiplier tmp279 (W256.of_int R));
     usr_res <- (PurePrimops.mulmod usr_res usr_factorMultiplier (W256.of_int R));
-    
-    sigma3_z <@ Primops.mload(PROOF_STATE_POLYS_3_OPENING_AT_Z_SLOT);
-    _22 <- (PurePrimops.addmod sigma3_z usr_gamma (W256.of_int R));
+    tmp280 <@ Primops.mload(PROOF_STATE_POLYS_3_OPENING_AT_Z_SLOT);
+    _22 <- (PurePrimops.addmod tmp280 usr_gamma (W256.of_int R));
     usr_res <- (PurePrimops.mulmod usr_res _22 (W256.of_int R));
     usr_res <- ((W256.of_int R) - usr_res);
-    
-    l0AtZ <@ Primops.mload(STATE_L_0_AT_Z_SLOT);
-    a5 <@ Primops.mload(STATE_POWER_OF_ALPHA_5_SLOT);
-    l0AtZ <- (PurePrimops.mulmod l0AtZ a5 (W256.of_int R));
-    _26 <- ((W256.of_int R) - l0AtZ);
+    usr_l0AtZ <@ Primops.mload(STATE_L_0_AT_Z_SLOT);
+    tmp282 <@ Primops.mload(STATE_POWER_OF_ALPHA_5_SLOT);
+    usr_l0AtZ <- (PurePrimops.mulmod usr_l0AtZ tmp282 (W256.of_int R));
+    _26 <- ((W256.of_int R) - usr_l0AtZ);
     usr_res <- (PurePrimops.addmod usr_res _26 (W256.of_int R));
-
     return usr_res;
   }
 
-  (* var a4, a5, b, g : Fr *)
-  (* var zp_z0, l0_z : Fr *)
-  (* var s0_z, s1_z, s2_z, s3_z : Fr *)
-  (* var a_z, b_z, c_z : Fr *)
- 
-  (* proc high() : Fr = { *)
-  (*   var s0BGa, s1BGb, s2BGc, s3G : Fr; *)
-
-  (*   s0BGa <- s0_z * b + g + a_z; *)
-  (*   s1BGb <- s1_z * b + g + b_z; *)
-  (*   s2BGc <- s2_z * b + g + c_z; *)
-  (*   s3G   <- s3_z + g; *)
+  proc low1(): uint256 = {
+    var usr_res, _alpha4, _zperm_zOmega, usr_gamma, usr_beta, usr_factorMultiplier, _sigma0_z, _a_z, _sigma1_z, _b_z, _sigma2_z, _c_z, _sigma3_z, _22, usr_l0AtZ, _alpha5, _26;
+    _alpha4 <@ Primops.mload(STATE_POWER_OF_ALPHA_4_SLOT);
+    _zperm_zOmega <@ Primops.mload(PROOF_COPY_PERMUTATION_GRAND_PRODUCT_OPENING_AT_Z_OMEGA_SLOT);
+    usr_gamma <@ Primops.mload(STATE_GAMMA_SLOT);
+    usr_beta <@ Primops.mload(STATE_BETA_SLOT);
+    _sigma0_z <@ Primops.mload(PROOF_COPY_PERMUTATION_POLYS_0_OPENING_AT_Z_SLOT);
+    _a_z <@ Primops.mload(PROOF_STATE_POLYS_0_OPENING_AT_Z_SLOT);
+    _sigma1_z <@ Primops.mload(PROOF_COPY_PERMUTATION_POLYS_1_OPENING_AT_Z_SLOT);
+    _b_z <@ Primops.mload(PROOF_STATE_POLYS_1_OPENING_AT_Z_SLOT);
+    _sigma2_z <@ Primops.mload(PROOF_COPY_PERMUTATION_POLYS_2_OPENING_AT_Z_SLOT);
+    _c_z <@ Primops.mload(PROOF_STATE_POLYS_2_OPENING_AT_Z_SLOT);
+    _sigma3_z <@ Primops.mload(PROOF_STATE_POLYS_3_OPENING_AT_Z_SLOT);
+    usr_l0AtZ <@ Primops.mload(STATE_L_0_AT_Z_SLOT);
+    _alpha5 <@ Primops.mload(STATE_POWER_OF_ALPHA_5_SLOT);
     
-  (*   return (-(a4 * zp_z0 * s0BGa * s1BGb * s2BGc * s3G)) - (a5 * l0_z); *)
-  (* } *)
- 
-  (* var _a4, _a5, _b, _g : int *)
-  (* var _zp_z0, _l0_z : int *)
-  (* var _s0_z, _s1_z, _s2_z, _s3_z : int *)
-  (* var _a_z, _b_z, _c_z : int *)
-  
-  (* proc mid() : int = { *)
-  (*   var s0BGa, s1BGb, s2BGc, s3G : int; *)
+    usr_res <- (PurePrimops.mulmod _zperm_zOmega _alpha4 (W256.of_int R));
+    usr_factorMultiplier <- (PurePrimops.mulmod _sigma0_z usr_beta (W256.of_int R));
+    usr_factorMultiplier <- (PurePrimops.addmod usr_factorMultiplier usr_gamma (W256.of_int R));
+    usr_factorMultiplier <- (PurePrimops.addmod usr_factorMultiplier _a_z (W256.of_int R));
+    usr_res <- (PurePrimops.mulmod usr_res usr_factorMultiplier (W256.of_int R));
+    usr_factorMultiplier <- (PurePrimops.mulmod _sigma1_z usr_beta (W256.of_int R));
+    usr_factorMultiplier <- (PurePrimops.addmod usr_factorMultiplier usr_gamma (W256.of_int R));
+    usr_factorMultiplier <- (PurePrimops.addmod usr_factorMultiplier _b_z (W256.of_int R));
+    usr_res <- (PurePrimops.mulmod usr_res usr_factorMultiplier (W256.of_int R));
+    usr_factorMultiplier <- (PurePrimops.mulmod _sigma2_z usr_beta (W256.of_int R));
+    usr_factorMultiplier <- (PurePrimops.addmod usr_factorMultiplier usr_gamma (W256.of_int R));
+    usr_factorMultiplier <- (PurePrimops.addmod usr_factorMultiplier _c_z (W256.of_int R));
+    usr_res <- (PurePrimops.mulmod usr_res usr_factorMultiplier (W256.of_int R));
+    _22 <- (PurePrimops.addmod _sigma3_z usr_gamma (W256.of_int R));
+    usr_res <- (PurePrimops.mulmod usr_res _22 (W256.of_int R));
+    usr_res <- ((W256.of_int R) - usr_res);
+    usr_l0AtZ <- (PurePrimops.mulmod usr_l0AtZ _alpha5 (W256.of_int R));
+    _26 <- ((W256.of_int R) - usr_l0AtZ);
+    usr_res <- (PurePrimops.addmod usr_res _26 (W256.of_int R));
+    return usr_res;
+  }
 
-  (*   s0BGa <- (_s0_z * _b + _g + _a_z)%%R; *)
-  (*   s1BGb <- (_s1_z * _b + _g + _b_z)%%R; *)
-  (*   s2BGc <- (_s2_z * _b + _g + _c_z)%%R; *)
-  (*   s3G   <- (_s3_z + _g)%%R; *)
+  proc low2(): uint256 = {
+    var usr_res, _alpha4, _zperm_zOmega, usr_gamma, usr_beta, usr_factorMultiplier, _sigma0_z, _a_z, _sigma1_z, _b_z, _sigma2_z, _c_z, _sigma3_z, usr_l0AtZ, _alpha5, _26;
+    var s0BGa, s1BGb, s2BGc, s3G;
+    
+    _alpha4 <@ Primops.mload(STATE_POWER_OF_ALPHA_4_SLOT);
+    _zperm_zOmega <@ Primops.mload(PROOF_COPY_PERMUTATION_GRAND_PRODUCT_OPENING_AT_Z_OMEGA_SLOT);
+    usr_gamma <@ Primops.mload(STATE_GAMMA_SLOT);
+    usr_beta <@ Primops.mload(STATE_BETA_SLOT);
+    _sigma0_z <@ Primops.mload(PROOF_COPY_PERMUTATION_POLYS_0_OPENING_AT_Z_SLOT);
+    _a_z <@ Primops.mload(PROOF_STATE_POLYS_0_OPENING_AT_Z_SLOT);
+    _sigma1_z <@ Primops.mload(PROOF_COPY_PERMUTATION_POLYS_1_OPENING_AT_Z_SLOT);
+    _b_z <@ Primops.mload(PROOF_STATE_POLYS_1_OPENING_AT_Z_SLOT);
+    _sigma2_z <@ Primops.mload(PROOF_COPY_PERMUTATION_POLYS_2_OPENING_AT_Z_SLOT);
+    _c_z <@ Primops.mload(PROOF_STATE_POLYS_2_OPENING_AT_Z_SLOT);
+    _sigma3_z <@ Primops.mload(PROOF_STATE_POLYS_3_OPENING_AT_Z_SLOT);
+    usr_l0AtZ <@ Primops.mload(STATE_L_0_AT_Z_SLOT);
+    _alpha5 <@ Primops.mload(STATE_POWER_OF_ALPHA_5_SLOT);
+    
+    usr_res <- (PurePrimops.mulmod _zperm_zOmega _alpha4 (W256.of_int R));
+    
+    s0BGa <- (PurePrimops.mulmod _sigma0_z usr_beta (W256.of_int R));
+    s0BGa <- (PurePrimops.addmod s0BGa usr_gamma (W256.of_int R));
+    s0BGa <- (PurePrimops.addmod s0BGa _a_z (W256.of_int R));
 
-  (*   return ((R - (_a4 * _zp_z0 * s0BGa * s1BGb * s2BGc * s3G)) + (R - (_a5 * _l0_z)))%%R; *)
-  (* }   *)
+    usr_factorMultiplier <- s0BGa;
+    usr_res <- (PurePrimops.mulmod usr_res usr_factorMultiplier (W256.of_int R));
+    
+    s1BGb <- (PurePrimops.mulmod _sigma1_z usr_beta (W256.of_int R));
+    s1BGb <- (PurePrimops.addmod s1BGb usr_gamma (W256.of_int R));
+    s1BGb <- (PurePrimops.addmod s1BGb _b_z (W256.of_int R));
+
+    usr_factorMultiplier <- s1BGb;
+    usr_res <- (PurePrimops.mulmod usr_res usr_factorMultiplier (W256.of_int R));
+
+    s2BGc <- (PurePrimops.mulmod _sigma2_z usr_beta (W256.of_int R));
+    s2BGc <- (PurePrimops.addmod s2BGc usr_gamma (W256.of_int R));
+    s2BGc <- (PurePrimops.addmod s2BGc _c_z (W256.of_int R));
+
+    usr_factorMultiplier <- s2BGc;
+    usr_res <- (PurePrimops.mulmod usr_res usr_factorMultiplier (W256.of_int R));
+
+    s3G   <- (PurePrimops.addmod _sigma3_z usr_gamma (W256.of_int R));
+    usr_res <- (PurePrimops.mulmod usr_res s3G (W256.of_int R));
+    
+    usr_res <- ((W256.of_int R) - usr_res);
+    usr_l0AtZ <- (PurePrimops.mulmod usr_l0AtZ _alpha5 (W256.of_int R));
+    _26 <- ((W256.of_int R) - usr_l0AtZ);
+    usr_res <- (PurePrimops.addmod usr_res _26 (W256.of_int R));
+    return usr_res;
+  }
+
+  proc low3(): uint256 = {
+    var usr_res1, usr_res2, _alpha4, _zperm_zOmega, usr_gamma, usr_beta, _sigma0_z, _a_z, _sigma1_z, _b_z, _sigma2_z, _c_z, _sigma3_z, usr_l0AtZ, _alpha5;
+    var s0BGa, s1BGb, s2BGc, s3G;
+    var inv1, inv2;
+    
+    _alpha4 <@ Primops.mload(STATE_POWER_OF_ALPHA_4_SLOT);
+    _zperm_zOmega <@ Primops.mload(PROOF_COPY_PERMUTATION_GRAND_PRODUCT_OPENING_AT_Z_OMEGA_SLOT);
+    usr_gamma <@ Primops.mload(STATE_GAMMA_SLOT);
+    usr_beta <@ Primops.mload(STATE_BETA_SLOT);
+    _sigma0_z <@ Primops.mload(PROOF_COPY_PERMUTATION_POLYS_0_OPENING_AT_Z_SLOT);
+    _a_z <@ Primops.mload(PROOF_STATE_POLYS_0_OPENING_AT_Z_SLOT);
+    _sigma1_z <@ Primops.mload(PROOF_COPY_PERMUTATION_POLYS_1_OPENING_AT_Z_SLOT);
+    _b_z <@ Primops.mload(PROOF_STATE_POLYS_1_OPENING_AT_Z_SLOT);
+    _sigma2_z <@ Primops.mload(PROOF_COPY_PERMUTATION_POLYS_2_OPENING_AT_Z_SLOT);
+    _c_z <@ Primops.mload(PROOF_STATE_POLYS_2_OPENING_AT_Z_SLOT);
+    _sigma3_z <@ Primops.mload(PROOF_STATE_POLYS_3_OPENING_AT_Z_SLOT);
+    usr_l0AtZ <@ Primops.mload(STATE_L_0_AT_Z_SLOT);
+    _alpha5 <@ Primops.mload(STATE_POWER_OF_ALPHA_5_SLOT);
+    
+    usr_res1 <- (PurePrimops.mulmod _zperm_zOmega _alpha4 (W256.of_int R));
+    
+    s0BGa <- (PurePrimops.mulmod _sigma0_z usr_beta (W256.of_int R));
+    s0BGa <- (PurePrimops.addmod s0BGa usr_gamma (W256.of_int R));
+    s0BGa <- (PurePrimops.addmod s0BGa _a_z (W256.of_int R));
+
+    usr_res1 <- (PurePrimops.mulmod usr_res1 s0BGa (W256.of_int R));
+    
+    s1BGb <- (PurePrimops.mulmod _sigma1_z usr_beta (W256.of_int R));
+    s1BGb <- (PurePrimops.addmod s1BGb usr_gamma (W256.of_int R));
+    s1BGb <- (PurePrimops.addmod s1BGb _b_z (W256.of_int R));
+
+    usr_res1 <- (PurePrimops.mulmod usr_res1 s1BGb (W256.of_int R));
+
+    s2BGc <- (PurePrimops.mulmod _sigma2_z usr_beta (W256.of_int R));
+    s2BGc <- (PurePrimops.addmod s2BGc usr_gamma (W256.of_int R));
+    s2BGc <- (PurePrimops.addmod s2BGc _c_z (W256.of_int R));
+
+    usr_res1 <- (PurePrimops.mulmod usr_res1 s2BGc (W256.of_int R));
+
+    s3G   <- (PurePrimops.addmod _sigma3_z usr_gamma (W256.of_int R));
+    usr_res1 <- (PurePrimops.mulmod usr_res1 s3G (W256.of_int R));
+    inv1 <- ((W256.of_int R) - usr_res1);
+    
+    usr_res2 <- (PurePrimops.mulmod usr_l0AtZ _alpha5 (W256.of_int R));
+    inv2 <- ((W256.of_int R) - usr_res2);
+
+    return (PurePrimops.addmod inv1 inv2 (W256.of_int R));
+  }
+
+  proc low(): uint256 = {
+    var usr_res1, usr_res2, _alpha4, _zperm_zOmega, usr_gamma, usr_beta, _sigma0_z, _a_z, _sigma1_z, _b_z, _sigma2_z, _c_z, _sigma3_z, usr_l0AtZ, _alpha5;
+    var s0BGa, s1BGb, s2BGc, s3G;
+    var inv1, inv2;
+    
+    _alpha4 <@ Primops.mload(STATE_POWER_OF_ALPHA_4_SLOT);
+    _zperm_zOmega <@ Primops.mload(PROOF_COPY_PERMUTATION_GRAND_PRODUCT_OPENING_AT_Z_OMEGA_SLOT);
+    usr_gamma <@ Primops.mload(STATE_GAMMA_SLOT);
+    usr_beta <@ Primops.mload(STATE_BETA_SLOT);
+    _sigma0_z <@ Primops.mload(PROOF_COPY_PERMUTATION_POLYS_0_OPENING_AT_Z_SLOT);
+    _a_z <@ Primops.mload(PROOF_STATE_POLYS_0_OPENING_AT_Z_SLOT);
+    _sigma1_z <@ Primops.mload(PROOF_COPY_PERMUTATION_POLYS_1_OPENING_AT_Z_SLOT);
+    _b_z <@ Primops.mload(PROOF_STATE_POLYS_1_OPENING_AT_Z_SLOT);
+    _sigma2_z <@ Primops.mload(PROOF_COPY_PERMUTATION_POLYS_2_OPENING_AT_Z_SLOT);
+    _c_z <@ Primops.mload(PROOF_STATE_POLYS_2_OPENING_AT_Z_SLOT);
+    _sigma3_z <@ Primops.mload(PROOF_STATE_POLYS_3_OPENING_AT_Z_SLOT);
+    usr_l0AtZ <@ Primops.mload(STATE_L_0_AT_Z_SLOT);
+    _alpha5 <@ Primops.mload(STATE_POWER_OF_ALPHA_5_SLOT);
+    
+    s0BGa <- (PurePrimops.mulmod _sigma0_z usr_beta (W256.of_int R));
+    s0BGa <- (PurePrimops.addmod s0BGa usr_gamma (W256.of_int R));
+    s0BGa <- (PurePrimops.addmod s0BGa _a_z (W256.of_int R));
+    
+    s1BGb <- (PurePrimops.mulmod _sigma1_z usr_beta (W256.of_int R));
+    s1BGb <- (PurePrimops.addmod s1BGb usr_gamma (W256.of_int R));
+    s1BGb <- (PurePrimops.addmod s1BGb _b_z (W256.of_int R));
+
+    s2BGc <- (PurePrimops.mulmod _sigma2_z usr_beta (W256.of_int R));
+    s2BGc <- (PurePrimops.addmod s2BGc usr_gamma (W256.of_int R));
+    s2BGc <- (PurePrimops.addmod s2BGc _c_z (W256.of_int R));
+
+    s3G   <- (PurePrimops.addmod _sigma3_z usr_gamma (W256.of_int R));
+
+    usr_res1 <- (PurePrimops.mulmod _zperm_zOmega _alpha4 (W256.of_int R));
+    usr_res1 <- (PurePrimops.mulmod usr_res1 s0BGa (W256.of_int R));
+    usr_res1 <- (PurePrimops.mulmod usr_res1 s1BGb (W256.of_int R));
+    usr_res1 <- (PurePrimops.mulmod usr_res1 s2BGc (W256.of_int R));
+    usr_res1 <- (PurePrimops.mulmod usr_res1 s3G (W256.of_int R));
+    inv1 <- ((W256.of_int R) - usr_res1);
+    
+    usr_res2 <- (PurePrimops.mulmod usr_l0AtZ _alpha5 (W256.of_int R));
+    inv2 <- ((W256.of_int R) - usr_res2);
+
+    return (PurePrimops.addmod inv1 inv2 (W256.of_int R));
+  }
+    
+  proc mid() : int = {
+    var s0BGa, s1BGb, s2BGc, s3G, inv1, inv2;
+    
+    s0BGa <- (sigma0_z * Beta + Gamma + a_z)%%R;
+    s1BGb <- (sigma1_z * Beta + Gamma + b_z)%%R;
+    s2BGc <- (sigma2_z * Beta + Gamma + c_z)%%R;
+    s3G   <- (sigma3_z + Gamma)%%R;
+
+    inv1 <- R - (Alpha4 * zperm_zO * s0BGa * s1BGb * s2BGc * s3G)%%R;
+    inv2 <- R - (Alpha5 * l0_z)%%R;
+    
+    return (inv1 + inv2)%%R;
+  }
 }.
 
-lemma permutationQuotientContribution_extracted_equiv_low :
-equiv [Verifier.usr_permutationQuotientContribution ~ PermutationQuotientContribution.low :
-      ={arg, glob PermutationQuotientContribution} ==> ={res, glob PermutationQuotientContribution}].
+section Lol.
+local lemma extracted_equiv_low0 :
+     equiv [Verifier.usr_permutationQuotientContribution ~ M.low0 :
+           ={arg, glob M} ==> ={res, glob M}].
 proof. proc.
-inline *; wp; skip; progress; smt ().
+  inline *; wp; skip; progress; smt ().
 qed.
 
+local lemma low0_equiv_low1 :
+     equiv [M.low0 ~ M.low1 : ={arg, glob M} ==> ={res, glob M}].
+proof. proc.
+  inline *; wp; skip; progress; smt ().
+qed.
 
-(* op permutationQuotientContribution_Mspec *)
-(*   (A4 A5 zperm_zO L0_z *)
-(*    sigma0_z sigma1_z sigma2_z sigma3_z *)
-(*    G B *)
-(*    a_z b_z c_z *)
-(*    rs : int) : bool = *)
-(*   let s0BGa = (sigma0_z * B + G + a_z)%%r in let s1BGb = (sigma1_z * B + G + b_z)%%r in *)
-(*   let s2BGc = (sigma2_z * B + G + c_z)%%r in let s3G   = (sigma3_z + G)%%r in *)
-(*   rs = ((r - (A4 * zperm_zO * s0BGa * s1BGb * s2BGc * s3G))%%r + (r - (A5 * L0_z)))%%r. *)
+local lemma low1_equiv_low2 :
+     equiv [M.low1 ~ M.low2 : ={arg, glob M} ==> ={res, glob M}].
+proof. proc.
+  inline *; wp; skip; progress; smt ().
+qed.
 
-(* op permutationQuotientContribution_Hspec *)
-(*   (A zperm_zO L0_z *)
-(*    sigma0_z sigma1_z sigma2_z sigma3_z *)
-(*    G B *)
-(*    a_z b_z c_z *)
-(*    rs : Fr) : bool = *)
-(*   let s0BGa = sigma0_z * B + G + a_z in let s1BGb = sigma1_z * B + G + b_z in *)
-(*   let s2BGc = sigma2_z * B + G + c_z in let s3G   = sigma3_z + G in *)
-(*   rs = (-(A^4 * zperm_zO * s0BGa * s1BGb * s2BGc * s3G)) - (A^5 * L0_z). *)
+local lemma low2_equiv_low3 :
+     equiv [M.low2 ~ M.low3 : ={arg, glob M} ==> ={res, glob M}].
+proof. proc.
+  inline *; wp; skip; progress; smt ().
+qed.
+
+local lemma low3_equiv_low :
+     equiv [M.low3 ~ M.low : ={arg, glob M} ==> ={res, glob M}].
+proof. proc.
+  inline *; wp; skip; progress; smt ().
+qed.
+
+lemma extracted_equiv_low :
+     equiv [Verifier.usr_permutationQuotientContribution ~ M.low :
+           ={arg, glob M} ==> ={res, glob M}].
+proof.
+transitivity M.low0 (={arg, glob M} ==> ={res, glob M}) (={arg, glob M} ==> ={res, glob M}); progress.
+exists Primops.memory{2}. progress. apply extracted_equiv_low0.
+transitivity M.low1 (={arg, glob M} ==> ={res, glob M}) (={arg, glob M} ==> ={res, glob M}); progress.
+exists Primops.memory{2}. progress. apply  low0_equiv_low1.
+transitivity M.low2 (={arg, glob M} ==> ={res, glob M}) (={arg, glob M} ==> ={res, glob M}); progress.
+exists Primops.memory{2}. progress. apply low1_equiv_low2.
+transitivity M.low3 (={arg, glob M} ==> ={res, glob M}) (={arg, glob M} ==> ={res, glob M}); progress.
+exists Primops.memory{2}. progress. apply low2_equiv_low3.
+apply low3_equiv_low.
+qed.
+
+end section Lol.
+
+lemma aux1 (n : int) : n %% R %% W256.modulus = n %% R. by smt(). qed.
+lemma aux2 : R %% W256.modulus = R. by smt(). qed.
+
+    
+lemma low_equiv_mid :
+equiv [M.low ~ M.mid :
+   ={arg, glob M} /\
+   Primops.memory{1} = memory /\
+   !Primops.reverted{1} /\
+   !Primops.reverted{2}
+   ==>
+   W256.to_uint res{1} = res{2}].
+proof. proc.
+
+seq 13 0 : (#pre /\
+  W256.to_uint _alpha4{1} = Alpha4 /\
+  W256.to_uint _alpha5{1} = Alpha5 /\
+  W256.to_uint _zperm_zOmega{1} = zperm_zO /\
+  W256.to_uint usr_gamma{1} = Gamma /\ 
+  W256.to_uint usr_beta{1} = Beta /\
+  W256.to_uint _sigma0_z{1} = sigma0_z /\
+  W256.to_uint _sigma1_z{1} = sigma1_z /\
+  W256.to_uint _sigma2_z{1} = sigma2_z /\
+  W256.to_uint _sigma3_z{1} = sigma3_z /\
+  W256.to_uint _a_z{1} = a_z /\
+  W256.to_uint _c_z{1} = c_z /\
+  W256.to_uint _b_z{1} = b_z /\
+  W256.to_uint usr_l0AtZ{1} = l0_z).
+call{1} (ConcretePrimops.mload_pspec memory STATE_POWER_OF_ALPHA_5_SLOT).
+call{1} (ConcretePrimops.mload_pspec memory STATE_L_0_AT_Z_SLOT).
+call{1} (ConcretePrimops.mload_pspec memory PROOF_STATE_POLYS_3_OPENING_AT_Z_SLOT).
+call{1} (ConcretePrimops.mload_pspec memory PROOF_STATE_POLYS_2_OPENING_AT_Z_SLOT).
+call{1} (ConcretePrimops.mload_pspec memory PROOF_COPY_PERMUTATION_POLYS_2_OPENING_AT_Z_SLOT).
+call{1} (ConcretePrimops.mload_pspec memory PROOF_STATE_POLYS_1_OPENING_AT_Z_SLOT).
+call{1} (ConcretePrimops.mload_pspec memory PROOF_COPY_PERMUTATION_POLYS_1_OPENING_AT_Z_SLOT).
+call{1} (ConcretePrimops.mload_pspec memory PROOF_STATE_POLYS_0_OPENING_AT_Z_SLOT).
+call{1} (ConcretePrimops.mload_pspec memory PROOF_COPY_PERMUTATION_POLYS_0_OPENING_AT_Z_SLOT).
+call{1} (ConcretePrimops.mload_pspec memory STATE_BETA_SLOT).
+call{1} (ConcretePrimops.mload_pspec memory STATE_GAMMA_SLOT).
+call{1} (ConcretePrimops.mload_pspec memory PROOF_COPY_PERMUTATION_GRAND_PRODUCT_OPENING_AT_Z_OMEGA_SLOT).
+call{1} (ConcretePrimops.mload_pspec memory STATE_POWER_OF_ALPHA_4_SLOT).
+skip; progress. 
+apply alpha4_mem. apply alpha5_mem. apply zperm_zO_mem. apply gamma_mem. apply beta_mem. apply sigma0_z_mem. apply sigma1_z_mem. apply sigma2_z_mem. apply sigma3_z_mem. apply a_z_mem. apply c_z_mem. apply b_z_mem. apply l0_z_mem.
+
+seq 10 4 : (#pre /\ W256.to_uint s0BGa{1} = s0BGa{2} /\ W256.to_uint s1BGb{1} = s1BGb{2} /\ W256.to_uint s2BGc{1} = s2BGc{2} /\ W256.to_uint s2BGc{1} = s2BGc{2} /\ W256.to_uint s3G{1} = s3G{2}). wp; skip; rewrite /addmod /mulmod; progress; rewrite !W256.of_uintK; by smt().
+
+seq 5 0 : (#pre /\ W256.to_uint usr_res1{1} = (Alpha4 * zperm_zO * s0BGa{2} * s1BGb{2} * s2BGc{2} * s3G{2})%%R). wp; skip; rewrite /addmod /mulmod; progress; rewrite !W256.of_uintK !aux2 !aux1; by smt().
+
+seq 1 1 : (#pre /\ W256.to_uint inv1{1} = inv1{2}).
+wp. skip. progress. rewrite -H14.
+have T: (R - to_uint usr_res1{1}) = (R - to_uint usr_res1{1}) %% W256.modulus. by smt().
+rewrite T -W256.of_uintK. smt(@W256).
+
+seq 1 0 : (#pre /\ W256.to_uint usr_res2{1} = (Alpha5 * l0_z)%%R). wp; skip; rewrite /addmod /mulmod; progress; rewrite !W256.of_uintK !aux2 !aux1; by smt().
+
+seq 1 1 : (#pre /\ W256.to_uint inv2{1} = inv2{2}).
+wp. skip. progress. rewrite -H15.
+have T: (R - to_uint usr_res2{1}) = (R - to_uint usr_res2{1}) %% W256.modulus. by smt().
+rewrite T -W256.of_uintK. smt(@W256).
+
+skip. progress. rewrite /addmod. progress. rewrite !W256.of_uintK !aux2 !aux1. by smt().
+qed. 
+end PermutationQuotientContribution.
